WIP

NuInstructions.thy
@@ -11,7 +11,7 @@ subsection \<open>Throw Exception\<close>
 text \<open>The opcode for throwing an exception is directly \<^term>\<open>Exception\<close>\<close>
 
 lemma (in std) throw_\<phi>app:
-  \<open>\<^bold>p\<^bold>r\<^bold>o\<^bold>c Exception \<lbrace> X \<longmapsto> Any \<^bold>t\<^bold>h\<^bold>r\<^bold>o\<^bold>w\<^bold>s X \<rbrace>\<close>
+  \<open>\<^bold>p\<^bold>r\<^bold>o\<^bold>c Exception \<lbrace> X \<longmapsto> 0 \<^bold>t\<^bold>h\<^bold>r\<^bold>o\<^bold>w\<^bold>s X \<rbrace>\<close>
   unfolding \<phi>Procedure_def by blast
 
 subsection \<open>Try-Catch\<close>
@@ -57,7 +57,7 @@ proc (in std) try'':
   argument X
   return YY
   throws EE2
-  \<medium_left_bracket> "__op_try__" F G \<medium_right_bracket> .. .
+  \<medium_left_bracket> "__op_try__" F G \<medium_right_bracket>. .
 
 proc (in std) try':
   assumes A: \<open>Union_the_Same_Or_Arbitrary_when_Var Z Y1 Y2\<close>
@@ -89,8 +89,9 @@ definition op_add :: "nat \<Rightarrow> 'VAL list \<Rightarrow> ('VAL,'RES_N,'RE
   where "op_add bits =
       \<phi>M_getV (\<tau>Int bits) (snd o V_int.dest) (\<lambda>val_a.
       \<phi>M_getV (\<tau>Int bits) (snd o V_int.dest) (\<lambda>val_b.
-      \<phi>M_Return [V_int.mk (bits, ((val_a + val_b) mod 2^bits))]
-  ))"
+      \<phi>M_getEnd ( 
+      Success [V_int.mk (bits, ((val_a + val_b) mod 2^bits))]
+  )))"
 
 
 lemma (in std) op_add:
@@ -111,21 +112,21 @@ definition op_sub :: "nat \<Rightarrow> 'VAL list \<Rightarrow> ('VAL,'RES_N,'RE
   where "op_sub bits =
       \<phi>M_getV (\<tau>Int bits) (snd o V_int.dest) (\<lambda>val_a.
       \<phi>M_getV (\<tau>Int bits) (snd o V_int.dest) (\<lambda>val_b.
-      \<phi>M_Return [V_int.mk (bits, ((2^bits + val_b - val_a) mod 2^bits))]
-  ))"
+      \<phi>M_getEnd (Success [V_int.mk (bits, ((2^bits + val_b - val_a) mod 2^bits))]
+  )))"
 
 definition op_udiv :: "nat \<Rightarrow> 'VAL list \<Rightarrow> ('VAL,'RES_N,'RES) proc"
   where "op_udiv bits =
       \<phi>M_getV (\<tau>Int bits) (snd o V_int.dest) (\<lambda>val_a.
       \<phi>M_getV (\<tau>Int bits) (snd o V_int.dest) (\<lambda>val_b.
-      \<phi>M_Return [V_int.mk (bits, (val_b div val_a))]
+      \<phi>M_getEnd (Success [V_int.mk (bits, (val_b div val_a))])
   ))"
 
 definition op_lt :: "nat \<Rightarrow> 'VAL list \<Rightarrow> ('VAL,'RES_N,'RES) proc"
   where "op_lt bits =
       \<phi>M_getV (\<tau>Int bits) (snd o V_int.dest) (\<lambda>val_a.
       \<phi>M_getV (\<tau>Int bits) (snd o V_int.dest) (\<lambda>val_b.
-      \<phi>M_Return [V_int.mk (1, (if val_b < val_a then 1 else 0))]
+      \<phi>M_getEnd (Success [V_int.mk (1, (if val_b < val_a then 1 else 0))])
   ))"
 
 
@@ -133,36 +134,36 @@ definition op_le :: "nat \<Rightarrow> 'VAL list \<Rightarrow> ('VAL,'RES_N,'RES
   where "op_le bits =
       \<phi>M_getV (\<tau>Int bits) (snd o V_int.dest) (\<lambda>val_a.
       \<phi>M_getV (\<tau>Int bits) (snd o V_int.dest) (\<lambda>val_b.
-      \<phi>M_Return [V_int.mk (1, (if val_b \<le> val_a then 1 else 0))]
+      \<phi>M_getEnd (Success [V_int.mk (1, (if val_b \<le> val_a then 1 else 0))])
   ))"
 
 
 definition op_not :: "'VAL list \<Rightarrow> ('VAL,'RES_N,'RES) proc"
   where "op_not =
     \<phi>M_getV (\<tau>Int 1) (snd o V_int.dest) (\<lambda>v.
-    \<phi>M_Return [V_int.mk (1, 1 - v)]
+    \<phi>M_getEnd (Success [V_int.mk (1, 1 - v)])
   )"
 
 definition op_and :: "'VAL list \<Rightarrow> ('VAL,'RES_N,'RES) proc"
   where "op_and =
     \<phi>M_getV (\<tau>Int 1) (snd o V_int.dest) (\<lambda>v.
     \<phi>M_getV (\<tau>Int 1) (snd o V_int.dest) (\<lambda>u.
-    \<phi>M_Return [V_int.mk (1, v+u-1)]
+    \<phi>M_getEnd (Success [V_int.mk (1, v+u-1)])
   ))"
 
 definition op_or :: "'VAL list \<Rightarrow> ('VAL,'RES_N,'RES) proc"
   where "op_or =
     \<phi>M_getV (\<tau>Int 1) (snd o V_int.dest) (\<lambda>v.
     \<phi>M_getV (\<tau>Int 1) (snd o V_int.dest) (\<lambda>u.
-    \<phi>M_Return [V_int.mk (1, min 1 (v+u))]
+    \<phi>M_getEnd (Success [V_int.mk (1, min 1 (v+u))])
   ))"
 
 definition op_equal :: "'TY \<Rightarrow> 'VAL list \<Rightarrow> ('VAL,'RES_N,'RES) proc"
   where "op_equal TY =
     \<phi>M_getV TY id (\<lambda>v.
-    \<phi>M_getV TY id (\<lambda>u vs.
-    (\<lambda>res. \<phi>M_assert (Can_EqCompare res v u) res) \<ggreater>
-    \<phi>M_Return [V_int.mk (1, (if EqCompare v u then 1 else 0))] vs
+    \<phi>M_getV TY id (\<lambda>u.
+    \<phi>M_getEnd ((\<lambda>res. \<phi>M_assert (Can_EqCompare res v u) res) \<ggreater>
+    Success [V_int.mk (1, (if EqCompare v u then 1 else 0))])
 ))"
 
 
@@ -209,8 +210,9 @@ definition \<phi>M_get_mem
 
 definition op_load_mem :: "'TY \<Rightarrow> 'VAL list \<Rightarrow> ('VAL,'RES_N,'RES) proc"
   where "op_load_mem TY =
-    \<phi>M_get_logptr TY (\<lambda>ptr vs.
-    \<phi>M_get_mem (memaddr.segment ptr) (memaddr.index ptr) (\<lambda>x. \<phi>M_Return [x] vs))"
+    \<phi>M_get_logptr TY (\<lambda>ptr.
+    \<phi>M_getEnd (
+    \<phi>M_get_mem (memaddr.segment ptr) (memaddr.index ptr) (\<lambda>x. Success [x])))"
 
 definition op_store_mem :: "'TY \<Rightarrow> 'VAL list \<Rightarrow> ('VAL,'RES_N,'RES) proc"
   where "op_store_mem TY =
@@ -519,18 +521,26 @@ definition op_get_var :: "varname \<Rightarrow> 'TY \<Rightarrow> ('VAL,'RES_N,'
   where "op_get_var vname TY = \<phi>M_get_var vname TY (\<lambda>x. Success [x])"
 
 definition op_set_var :: "varname \<Rightarrow> 'TY \<Rightarrow> 'VAL list \<Rightarrow> ('VAL,'RES_N,'RES) proc"
-  where "op_set_var vname TY = (\<lambda>v. \<phi>M_get_var vname TY (\<lambda>_.
-            \<phi>M_assert (v \<in> Well_Type TY) \<ggreater> \<phi>M_set_res_entry R_var.updt (\<lambda>f. f(vname := Some v))))"
+  where "op_set_var vname TY =
+          \<phi>M_getV TY id (\<lambda>v.
+          \<phi>M_getEnd (
+          \<phi>M_get_var vname TY (\<lambda>_.
+          \<phi>M_set_res_entry R_var.updt (\<lambda>f. f(vname := Some v)))))"
 
-definition op_free_var :: "varname \<Rightarrow> (unit,'RES_N,'RES) proc"
+definition op_free_var :: "varname \<Rightarrow> ('VAL,'RES_N,'RES) proc"
   where "op_free_var vname = \<phi>M_set_res_entry R_var.updt (\<lambda>f. f(vname := None))"
 
-definition op_var_scope' :: "'TY \<Rightarrow> 'VAL \<Rightarrow> (varname \<Rightarrow> ('ret::value,'RES_N,'RES) proc) \<Rightarrow> ('ret,'RES_N,'RES) proc"
-  where "op_var_scope' TY v F =
+definition op_var_scope' :: "'TY
+                          \<Rightarrow> (varname \<Rightarrow> ('VAL,'RES_N,'RES) proc)
+                          \<Rightarrow> 'VAL list \<Rightarrow> ('VAL,'RES_N,'RES) proc"
+  where "op_var_scope' TY F =
+    \<phi>M_getV TY id (\<lambda>v.
+    \<phi>M_getEnd (
     \<phi>M_get_res R_var.get (\<lambda>f.
     let vname = (@vname. f vname = None) in
     \<phi>M_set_res_entry R_var.updt (\<lambda>f. f(vname := Some v)) \<ggreater>
-    F vname)"
+    F vname
+  )))"
 
 lemma (in std) \<phi>M_get_var[\<phi>reason!]:
   \<open>v \<in> Well_Type TY
@@ -588,16 +598,17 @@ end
 lemma (in std) op_set_var''_\<phi>app:
    \<open>\<^bold>p\<^bold>r\<^bold>e\<^bold>m\<^bold>i\<^bold>s\<^bold>e v \<in> Well_Type TY
 \<Longrightarrow> \<^bold>p\<^bold>r\<^bold>e\<^bold>m\<^bold>i\<^bold>s\<^bold>e u \<in> Well_Type TY
-\<Longrightarrow> \<^bold>p\<^bold>r\<^bold>o\<^bold>c op_set_var vname TY rawv \<lbrace> v \<Ztypecolon> Var vname Identity\<heavy_comma> u \<Ztypecolon> Val rawv Identity \<longmapsto> \<lambda>_. u \<Ztypecolon> Var vname Identity \<rbrace>\<close>
+\<Longrightarrow> \<^bold>p\<^bold>r\<^bold>o\<^bold>c op_set_var vname TY [rawv] \<lbrace> v \<Ztypecolon> Var vname Identity\<heavy_comma> u \<Ztypecolon> Val rawv Identity \<longmapsto> \<lambda>_. u \<Ztypecolon> Var vname Identity \<rbrace>\<close>
   unfolding op_set_var_def Premise_def
-  by (clarsimp simp add: \<phi>expns, rule \<phi>M_get_var, assumption, rule \<phi>M_set_var)
+  by (\<phi>reason, assumption, simp add: \<phi>expns, \<phi>reason)
 
 
 lemma (in std) op_var_scope':
    \<open>\<^bold>p\<^bold>r\<^bold>e\<^bold>m\<^bold>i\<^bold>s\<^bold>e v \<in> Well_Type TY
     \<Longrightarrow> (\<And>vname. \<^bold>p\<^bold>r\<^bold>o\<^bold>c F vname \<lbrace> X\<heavy_comma> v \<Ztypecolon> Var vname Identity \<longmapsto> Y \<^bold>t\<^bold>h\<^bold>r\<^bold>o\<^bold>w\<^bold>s E \<rbrace> )
-    \<Longrightarrow> \<^bold>p\<^bold>r\<^bold>o\<^bold>c op_var_scope' TY rawv F \<lbrace> X\<heavy_comma> v \<Ztypecolon> Val rawv Identity \<longmapsto> Y \<^bold>t\<^bold>h\<^bold>r\<^bold>o\<^bold>w\<^bold>s E \<rbrace>\<close>
+    \<Longrightarrow> \<^bold>p\<^bold>r\<^bold>o\<^bold>c op_var_scope' TY F [rawv] \<lbrace> X\<heavy_comma> v \<Ztypecolon> Val rawv Identity \<longmapsto> Y \<^bold>t\<^bold>h\<^bold>r\<^bold>o\<^bold>w\<^bold>s E \<rbrace>\<close>
   unfolding op_var_scope'_def Premise_def
+  apply (\<phi>reason)
   apply (simp add: \<phi>expns)
   unfolding \<phi>Procedure_def
   unfolding \<phi>M_set_res_entry_def \<phi>Procedure_def \<phi>M_get_res_def Let_def bind_def
@@ -611,7 +622,6 @@ lemma (in std) op_var_scope':
       unfolding sep_disj_fun_def by simp (meson someI t1)
     have t3[simp]: \<open>vars (SOME vname. vars vname = None) = None\<close>
       by (meson someI t1)
-
     show ?thesis
       apply (rule \<open>\<forall>a. _\<close>[of \<open>(SOME vname. vars vname = None)\<close>,
         THEN spec, THEN spec, THEN mp])
@@ -658,37 +668,42 @@ subsection \<open>Branches & Loops\<close>
 
 paragraph \<open>Non-Branching Selection\<close>
 
-definition op_sel :: "'VAL \<Rightarrow> 'VAL \<Rightarrow> 'VAL \<Rightarrow> ('VAL,'RES_N,'RES) proc"
-  where "op_sel vc b a = 
-    \<phi>M_getV (\<tau>Int 1) V_int.dest vc (\<lambda>c. Success (if snd c = 1 then a else b))"
+definition op_sel :: "'TY \<Rightarrow> 'VAL list \<Rightarrow> ('VAL,'RES_N,'RES) proc"
+  where "op_sel TY = 
+    \<phi>M_getV (\<tau>Int 1) V_int.dest (\<lambda>c.
+    \<phi>M_getV TY id (\<lambda>a.
+    \<phi>M_getV TY id (\<lambda>b.
+    \<phi>M_getEnd (
+    Success [if snd c = 1 then a else b]))))"
 
 paragraph \<open>Branch\<close>
 
-definition op_if :: "'VAL
-                  \<Rightarrow> ('ret::value,'RES_N,'RES) proc
-                  \<Rightarrow> ('ret,'RES_N,'RES) proc
-                  \<Rightarrow> ('ret,'RES_N,'RES) proc"
-  where "op_if vc brT brF =
-    \<phi>M_getV (\<tau>Int 1) V_int.dest vc (\<lambda>c. if snd c = 1 then brT else brF)"
+definition op_if :: "('VAL,'RES_N,'RES) proc
+                  \<Rightarrow> ('VAL,'RES_N,'RES) proc
+                  \<Rightarrow> 'VAL list
+                  \<Rightarrow> ('VAL,'RES_N,'RES) proc"
+  where "op_if brT brF =
+    \<phi>M_getV (\<tau>Int 1) V_int.dest (\<lambda>c.
+    \<phi>M_getEnd (if snd c = 1 then brT else brF))"
 
 paragraph \<open>While Loop\<close>
 
-inductive SemDoWhile :: "('VAL,'RES_N,'RES) proc \<Rightarrow> ('RES_N \<Rightarrow> 'RES) \<Rightarrow> (unit,'RES_N,'RES) state \<Rightarrow> bool" where
-  "f s = Success (V_int.mk (1,0)) res \<Longrightarrow> SemDoWhile f s (Success vs res)"
-| "f s = Success (V_int.mk (1,1)) res \<Longrightarrow> SemDoWhile f res s'' \<Longrightarrow> SemDoWhile f s s''"
+inductive SemDoWhile :: "('VAL,'RES_N,'RES) proc \<Rightarrow> ('RES_N \<Rightarrow> 'RES) \<Rightarrow> ('VAL,'RES_N,'RES) state \<Rightarrow> bool" where
+  "f s = Success [V_int.mk (1,0)] res \<Longrightarrow> SemDoWhile f s (Success [] res)"
+| "f s = Success [V_int.mk (1,1)] res \<Longrightarrow> SemDoWhile f res s'' \<Longrightarrow> SemDoWhile f s s''"
 | "f s = Exception e \<Longrightarrow> SemDoWhile f s (Exception e)"
 | "f s = PartialCorrect \<Longrightarrow> SemDoWhile f s PartialCorrect"
 | "f s = Fail \<Longrightarrow> SemDoWhile f s Fail"
 
-lemma "\<nexists> y. SemDoWhile (\<lambda>res. Success (V_int.mk (1,1)) res) res y"
+lemma "\<nexists> y. SemDoWhile (\<lambda>res. Success [V_int.mk (1,1)] res) res y"
   apply rule apply (elim exE) subgoal for y 
     thm SemDoWhile.induct
-    apply (induct "(\<lambda>res. Success (V_int.mk (1,1)) (res::'RES_N \<Rightarrow> 'RES))" res y
+    apply (induct "(\<lambda>res. Success [V_int.mk (1,1)] (res::'RES_N \<Rightarrow> 'RES))" res y
            rule: SemDoWhile.induct)
        apply simp_all
     done done
 
-definition op_do_while :: "('VAL,'RES_N,'RES) proc \<Rightarrow> (unit,'RES_N,'RES) proc" where
+definition op_do_while :: "('VAL,'RES_N,'RES) proc \<Rightarrow> ('VAL,'RES_N,'RES) proc" where
   "op_do_while f s = (if (\<exists>y. SemDoWhile f s y) then The (SemDoWhile f s) else PartialCorrect)"
 
 lemma SemDoWhile_deterministic:
@@ -697,7 +712,7 @@ lemma SemDoWhile_deterministic:
     shows "s1 = s2"
 proof -
   have "SemDoWhile c s s1 \<Longrightarrow> (\<forall>s2. SemDoWhile c s s2 \<longrightarrow> s1 = s2)"
-    apply (induct rule: SemDoWhile.induct) 
+    apply (induct rule: SemDoWhile.induct)
     by (subst SemDoWhile.simps, simp)+
   thus ?thesis
     using assms by simp
@@ -710,15 +725,15 @@ lemma SemDoWhile_deterministic2:
 
 paragraph \<open>Recursion\<close>
 
-inductive SemRec :: "(('arg \<Rightarrow> ('ret,'RES_N,'RES) proc) \<Rightarrow> 'arg \<Rightarrow> ('ret,'RES_N,'RES) proc)
-          \<Rightarrow> 'arg \<Rightarrow> ('RES_N \<Rightarrow> 'RES) \<Rightarrow> ('ret,'RES_N,'RES) state \<Rightarrow> bool"
+inductive SemRec :: "(('VAL list \<Rightarrow> ('VAL,'RES_N,'RES) proc) \<Rightarrow> 'VAL list \<Rightarrow> ('VAL,'RES_N,'RES) proc)
+            \<Rightarrow> 'VAL list \<Rightarrow> ('RES_N \<Rightarrow> 'RES) \<Rightarrow> ('VAL,'RES_N,'RES) state \<Rightarrow> bool"
 where
   SemRec_I0: "(\<And>g. F g x res = y) \<Longrightarrow> SemRec F x res y"
 | SemRec_IS: "SemRec (F o F) x res y \<Longrightarrow> SemRec F x res y"
 
 definition op_recursion :: "'TY list \<Rightarrow> 'TY list
-                         \<Rightarrow> (('arg \<Rightarrow> ('ret::value,'RES_N,'RES) proc) \<Rightarrow> 'arg \<Rightarrow> ('ret,'RES_N,'RES) proc)
-                         \<Rightarrow> 'arg \<Rightarrow> ('ret,'RES_N,'RES) proc"
+                         \<Rightarrow> (('VAL list \<Rightarrow> ('VAL,'RES_N,'RES) proc) \<Rightarrow> 'VAL list \<Rightarrow> ('VAL,'RES_N,'RES) proc)
+                         \<Rightarrow> 'VAL list \<Rightarrow> ('VAL,'RES_N,'RES) proc"
   where "op_recursion _ _ F x s = (if (\<exists>t. SemRec F x s t) then The (SemRec F x s) else PartialCorrect)"
 
 
