NuLLReps.thy
@@ -484,11 +484,11 @@ lemma [\<phi>reason 110 on \<open>\<^bold>s\<^bold>u\<^bold>b\<^bold>t\<^bold>y\
 
 subsubsection \<open>Synthesis Rules\<close>
 
-lemma [\<phi>reason on \<open>\<^bold>p\<^bold>r\<^bold>o\<^bold>c ?f \<lbrace> ?S1 \<longmapsto> \<lambda>_. ?S2\<heavy_comma> SYNTHESIS ?x \<Ztypecolon> Var ?var ?T \<^bold>t\<^bold>h\<^bold>r\<^bold>o\<^bold>w\<^bold>s ?E \<rbrace> \<^bold>@\<^bold>G\<^bold>O\<^bold>A\<^bold>L ?G\<close>]:
+lemma [\<phi>reason on \<open>\<^bold>p\<^bold>r\<^bold>o\<^bold>c ?f \<lbrace> ?S1 \<longmapsto> ?S2\<heavy_comma> SYNTHESIS ?x \<Ztypecolon> Var ?var ?T \<^bold>t\<^bold>h\<^bold>r\<^bold>o\<^bold>w\<^bold>s ?E \<rbrace> \<^bold>@\<^bold>G\<^bold>O\<^bold>A\<^bold>L ?G\<close>]:
   \<open> SUBGOAL G G'
 \<Longrightarrow> \<^bold>s\<^bold>u\<^bold>b\<^bold>t\<^bold>y\<^bold>p\<^bold>e S1 \<longmapsto> S2\<heavy_comma> \<blangle> x \<Ztypecolon> Var var T \<brangle> \<^bold>@\<^bold>G\<^bold>O\<^bold>A\<^bold>L G'
 \<Longrightarrow> SOLVE_SUBGOAL G'
-\<Longrightarrow> \<^bold>p\<^bold>r\<^bold>o\<^bold>c Success () \<lbrace> S1 \<longmapsto> \<lambda>_. S2\<heavy_comma> SYNTHESIS x \<Ztypecolon> Var var T \<rbrace> \<^bold>@\<^bold>G\<^bold>O\<^bold>A\<^bold>L G\<close>
+\<Longrightarrow> \<^bold>p\<^bold>r\<^bold>o\<^bold>c Success [] \<lbrace> S1 \<longmapsto> S2\<heavy_comma> SYNTHESIS x \<Ztypecolon> Var var T \<rbrace> \<^bold>@\<^bold>G\<^bold>O\<^bold>A\<^bold>L G\<close>
   unfolding GOAL_CTXT_def FOCUS_TAG_def Synthesis_def
   using "\<phi>cast" \<phi>reassemble_proc_final
   by (metis (no_types, lifting) \<phi>SKIP \<phi>apply_proc)
